\chapter{Dovetailing lemmas}

\dtone*
\begin{proof}
	\label{proof:dtone}
The proof can be carried out by simple rewriting. Given that:
\[dt(x,y)=\frac{(x+y)(x+y+1)}{2}+y\]
and consequently that:
\[dt(x+1,y)=\frac{(x+y+1)(x+y+2)}{2}+y\]
we have that
\[\begin{split}
	dt(x+1,y)-dt(x,y)&=\frac{(x+y+1)}{2}(\cancel{x+y}+2\cancel{-x-y})\\
                         &=x+y+1\\
\end{split}\]
Therefore:
\[dt(x+1,y) = dt(x,y) + x +y +1\]
\end{proof}


\dttwo*
\begin{proof}
		\label{proof:dttwo}
We can prove it by induction over $i$. 
\begin{description}
	\item[$i=0$] holds by substitution of $i$ and reflexivity.
	\item[$i=1$] holds by lemma \ref{dtone}.
	\item[$i=n+1$] The induction hypothesis is the following:
	\[dt(x+n,y)=dt(x,y)+n(x+y)+\sum_{j=0}^nj\]
	Therefore, we have that:
\[\begin{split}
dt(x+n+1,y)&=dt(x+n,y)+x+y+(n+1)\\
	&\overset{IH}{=}dt(x,y)+(n)(x+y)+\sum_{j=0}^nj+(x+y)+(n+1)\\
	&=dt(x,y)+(n+1)(x+y)+\sum_{j=0}^{n+1}j
\end{split}\]
\end{description}
\end{proof}

\dtcreat*
\begin{proof}
The proof can be carried out by simple rewriting. Given that:
\[dt(x,y)=\frac{(x+y)(x+y+1)}{2}+y\]
and consequently that:
\[dt(x,y+1)=\frac{(x+y+1)(x+y+2)}{2}+y+1\]
we have that
\[\begin{split}
dt(x+1,y)-dt(x,y)&=1+\frac{(x+y+1)}{2}(\cancel{x+y}+2\cancel{-x-y})\\
&=x+y+2\\
\end{split}\]
Therefore:
\[dt(x+1,y) = dt(x,y) + x +y +2\]
\end{proof}
